Deterministic LTS  (#128)
Deterministic labelled transition systems. 

* Add a subclass of deterministic lts
* Add function `ftrans l s` which picks a state `s'`  s.t. there exists transition `s --[l]--> s'` (if there is not transition returns `s`). Prove that for deterministic lts `ftrans` coincides with labelled transition relation. 
  Construction of `ftrans` requires choice operator on states --- so the type of LTS states now inherits from `choiceType`.
* Introduce `trace_from s ls` function to build a trace starting from state `s` following labels `ls`. 
* Prove reflection lemma for language of deterministic lts.

theories/concur/lts.v
@@ -1,5 +1,5 @@
 From RelationAlgebra Require Import lattice monoid rel.
-From mathcomp Require Import ssreflect ssrfun ssrbool ssrnat eqtype.
+From mathcomp Require Import ssreflect ssrfun ssrbool ssrnat eqtype choice.
 From mathcomp Require Import seq tuple path.
 From eventstruct Require Import utils relalg.
 
@@ -7,56 +7,82 @@ From eventstruct Require Import utils relalg.
 (* This file provides a theory of labelled transition systems (LTS),          *)
 (* traces and languages of LTS, and simulation relations between LTS.         *)
 (*                                                                            *)
-(*         ltsType L == a type of states of labelled transition system with   *)
-(*                      labels from L. Currently the library supports only    *)
-(*                      discrete states, i.e. the type of states should have  *)
-(*                      decidable equality.                                   *)
-(*             trans == transition relation of type L -> S -> S -> bool.      *)
-(*    s1 --[l]--> s2 == there exists a transition from s1 to s2 labelled by l.*)
-(*         s1 --> s2 == there exists a transition from s1 to s2.              *)
-(*        s1 -->? s2 == s1 is equal to s2 or s1 --> s2.                       *)
-(*        s1 -->+ s2 == there exists a non-empty sequence of steps            *)
-(*                      from s1 to s2.                                        *)
-(*        s1 -->* s2 == there exists a possibly empty sequence of steps       *)
-(*                      from s1 to s2.                                        *)
-(*            step S == a type of steps of the LTS.                           *)
-(*                   := { (lbl, src, dst) | src --[lbl]--> dst }.             *)
-(*         step_of H == given a proof of step property H : s --[l]--> s'      *)
-(*                      constructs a step { (l, s, s') | s --[l]--> s' }.     *)
-(*           trace S == a type of traces of the LTS, that is finite sequences *)
-(*                      of steps performed by the transition system.          *)
-(*                   := { tr : seq (step S) | dst tr[i] == src tr[i+1] }.     *)
-(*     [trace of ts] == a trace whose underlying sequence (value) is ts.      *)
-(*                      Coq must be able to infer a proof that ts satisfies   *)
-(*                      trace property (i.e the ends of steps should match).  *)
-(*           [trace] == empty trace.                                          *)
-(*       tr1 <+> tr2 == concatenation of traces tr1 ++ tr2 if tr1 and tr2     *)
-(*                      are adjoint, empty trace otherwise.                   *)
-(*          st <+ tr == cons of step st and trace tr if they are are adjoint, *)
-(*                      empty trace otherwise.                                *)
-(*          tr +> st == rcons of step st and trace tr if they are are adjoint,*)
-(*                      empty trace otherwise.                                *)
-(*         labels tr == a sequence of labels of a trace.                      *)
-(*       states s tr == a sequence of states of tr or [:: s] if tr is empty.  *)
-(*    fst_state s tr == the first state of tr or s is tr is empty.            *)
-(*    lst_state s tr == the last state of tr or s is tr is empty.             *)
-(*   adjoint tr1 tr2 == a relation asserting that two traces are adjoint,     *)
-(*                      meaning that the last state of tr1 is equal to        *)
-(*                      the first state of tr2.                               *)
-(*      trace_lang s == a (decidable) predicate defining a trace language     *)
-(*                      (a set of traces) of the LTS at the state s,          *)
-(*                      i.e. valid traces starting at the state s.            *)
-(*        lts_lang s == a predicate defining a language (a set of label       *)
-(*                      sequences) of the LTS at the state s.                 *)
+(*            ltsType L == a type of states of a labelled transition system   *)
+(*                         with labels from L. Currently the library supports *)
+(*                         only states with decidable equality and            *)
+(*                         choice operator, i.e. the type of states           *)
+(*                         inherets from choiceType.                          *)
+(*           dltsType L == a type of states of a deterministic labelled       *)
+(*                         transition system.                                 *)
+(*               ltrans == labelled transition relation of type               *)
+(*                         L -> S -> S -> bool.                               *)
+(*                trans == unlabelled transition relation of type             *)
+(*                         S -> S -> bool.                                    *)
+(*        has_trans s l == checks that there exists a transition from         *)
+(*                         state s by label l.                                *)
+(*           ftrans s l == if there exists transition from s by l then        *)
+(*                         picks some state s' reachable by this transition,  *)
+(*                         otherwise returns s.                               *)
+(*       s1 --[l]--> s2 == boolean relation asserting that there exists       *)
+(*                         a transition from s1 to s2 labelled by l.          *)
+(*            s1 --> s2 == boolean relation asserting that there exists       *)
+(*                         transition from s1 to s2.                          *)
+(*           s1 -->? s2 == propositional relation asserting that              *)
+(*                         s1 is equal to s2 or there exists a transition     *)
+(*                         from s1 to s2.                                     *)
+(*           s1 -->+ s2 == propositional relation asserting that there exists *)
+(*                         a non-empty sequence of steps from s1 to s2.       *)
+(*           s1 -->* s2 == propositional relation asserting that there exists *) 
+(*                         a possibly empty sequence of steps from s1 to s2.  *)
+(*                                                                            *)
+(* For an LTS we develop a theory of its (linear) traces.                     *)
+(*               step S == a type of steps of the LTS.                        *)
+(*                      := { (lbl, src, dst) | src --[lbl]--> dst }.          *)
+(*            step_of H == given a proof of step property H : s --[l]--> s'   *)
+(*                         constructs a step { (l, s, s') | s --[l]--> s' }.  *)
+(*              trace S == a type of traces of the LTS, i.e. finite sequences *) 
+(*                          of steps performed by the transition system.      *)
+(*                      := { tr : seq (step S) | dst tr[i] == src tr[i+1] }.  *)
+(*        [trace of ts] == a trace whose underlying sequence (value) is ts.   *)
+(*                         Coq must be able to infer a proof that ts          *)
+(*                         satisfies trace property.                          *)
+(*              [trace] == empty trace.                                       *)
+(*         [trace:: st] == singleton trace consisting of the step st.         *)
+(*       [trace? of ts] == a trace whose underlying sequence (value) is ts    *)
+(*                         if ts satisfies trace property,                    *)
+(*                         or empty trace otherwise.                          *)
+(* [trace from s by ls] == if the sequence of labels ls is accepted by LTS at *)
+(*                         state s then it returns a trace starting from s    *)
+(*                         with the labels equal to ls, otherwise empty trace.*)  
+(*          tr1 <+> tr2 == concatenation of traces tr1 ++ tr2 if tr1 and tr2  *)
+(*                         are adjoint, empty trace otherwise.                *)
+(*             st <+ tr == cons of step st and trace tr if they are adjoint,  *)
+(*                         empty trace otherwise.                             *)
+(*             tr +> st == rcons of step st and trace tr if they are adjoint, *)
+(*                         empty trace otherwise.                             *)
+(*            labels tr == a sequence of labels of a trace.                   *)
+(*          states s tr == a sequence of states of tr or [:: s]               *)
+(*                         if tr is empty.                                    *)
+(*       fst_state s tr == the first state of tr or s is tr is empty.         *)
+(*       lst_state s tr == the last state of tr or s is tr is empty.          *)
+(*      adjoint tr1 tr2 == a relation asserting that two traces are adjoint,  *)
+(*                         meaning that the last state of tr1 is equal to     *)
+(*                         the first state of tr2.                            *)
+(*         trace_lang s == a (boolean) predicate defining a trace language    *)
+(*                         (a set of traces) of the LTS at the state s,       *)
+(*                         i.e. valid traces starting at the state s.         *)
+(*           lts_lang s == a (propositional) predicate defining a language    *)
+(*                         (a set of label sequences) of the LTS              *)
+(*                         accepted at the state s.                           *)
 (*                                                                            *)
 (* We also develop a theory of simulations between transition systems.        *)
 (*           sim S T == a type of simulation relations between S and T.       *)
 (*         bisim S T == a type of bisimulation relations between S and T.     *)
 (* The following important lemmas about simulations are available.            *)
 (*    sim_lang R s t == if R is simulation and R s t holds then               *)
-(*                      lts_lang s ≦ lts_lang t.                              *)
-(*    sim_lang R s t == if R is simulation and R s t holds then               *)
-(*                      lts_lang s ≡ lts_lang t.                              *)
+(*                      lts_lang s is a subset of lts_lang t.                 *)
+(*  bisim_lang R s t == if R is bisimulation and R s t holds then             *)
+(*                      lts_lang s is equivalent to lts_lang t.               *)
 (*                                                                            *)
 (* The following notations can be used by importing corresponding module:     *)
 (* Import Mod.Syntax for Mod in {Simulation, Bisimulation}.                   *)
@@ -84,34 +110,36 @@ Reserved Notation "s1 '-->?' s2" (at level 55, right associativity).
 Reserved Notation "s1 '-->+' s2" (at level 55, right associativity).
 Reserved Notation "s1 '-->*' s2" (at level 55, right associativity).
 
-Module Export LTS.
-
 Section ExLab.
 Context {S L : Type}.
 
 (* TODO: remove copypaste from `rewriting_system.v` *)
-Definition exlab {S L : Type} (tr : L -> hrel S S) : hrel S S := 
-  fun s1 s2 => exists l, tr l s1 s2.
+Definition exlab {S L : Type} (ltr : L -> hrel S S) : hrel S S := 
+  fun s1 s2 => exists l, ltr l s1 s2.
 
 End ExLab.
+
+Module Export LTS.
 
 Module LTS.
 Section ClassDef. 
 
 Record mixin_of (S0 : Type) (L : Type)
-                (sb : Equality.class_of S0)
-                (S := Equality.Pack sb) := Mixin {
-  trans : L -> rel S;
+                (sb : Countable.class_of S0)
+                (S := Countable.Pack sb) := Mixin {
+  ltrans    : L -> rel S;
+  has_trans : L -> S -> bool;
+  _ : forall l s, reflect (exists s', ltrans l s s') (has_trans l s);
 }.
 
 Set Primitive Projections.
 Record class_of (S : Type) (L : Type) := Class {
-  base  : Equality.class_of S;
+  base  : Countable.class_of S;
   mixin : mixin_of L base;
 }.
 Unset Primitive Projections.
 
-Local Coercion base : class_of >-> Equality.class_of.
+Local Coercion base : class_of >-> Countable.class_of.
 
 Structure type (L : Type) := Pack { sort; _ : class_of sort L }.
 
@@ -123,18 +151,25 @@ Definition class := let: Pack _ c as cT' := cT return class_of (sort cT') L in c
 Definition clone c of phant_id class c := @Pack S c.
 
 Definition pack :=
-  fun bS b & phant_id (@Equality.class bS) b =>
+  fun bS b & phant_id (@Countable.class bS) b =>
   fun m => Pack (@Class S L b m).
 
 Definition eqType := @Equality.Pack cT class.
+Definition choiceType := @Choice.Pack cT class.
+Definition countType := @Countable.Pack cT class.
+
 End ClassDef.
 
 Module Export Exports.
-Coercion base : class_of >-> Equality.class_of.
+Coercion base : class_of >-> Countable.class_of.
 Coercion mixin : class_of >-> mixin_of.
 Coercion sort : type >-> Sortclass.
 Coercion eqType : type >-> Equality.type.
+Coercion choiceType : type >-> Choice.type.
+Coercion countType : type >-> Countable.type.
 Canonical eqType.
+Canonical choiceType.
+Canonical countType.
 End Exports.
 
 End LTS.
@@ -146,18 +181,147 @@ Notation LTSType S L m := (@LTS.pack S L _ _ id m).
 
 Section Def.
 Context {L : Type} (S : ltsType L).
+Implicit Types (l : L) (s : S).
 
-Definition trans : L -> rel S := LTS.trans (LTS.class S).
+Definition ltrans : L -> rel S := LTS.ltrans (LTS.class S).
+
+Definition has_trans : L -> S -> bool := LTS.has_trans (LTS.class S).
+
+Lemma has_transP l s : 
+  reflect (exists s', ltrans l s s') (has_trans l s).
+Proof. by rewrite /ltrans /has_trans; move: s; case: S=> ? [? []]. Qed. 
+
+Definition ftrans : L -> S -> S := 
+  fun l s => match @idP (has_trans l s) with 
+  | ReflectT pf => 
+     let exP := elimT (has_transP l s) pf in 
+     xchoose exP
+  | ReflectF pf => s 
+  end.
 
 End Def.
 
-Notation "s1 '--[' l ']-->' s2" := (trans l s1 s2) : lts_scope.
-Notation "s1 '-->' s2"  := (exlab trans)   : lts_scope.
-Notation "s1 '-->?' s2" := (exlab trans)^? : lts_scope.
-Notation "s1 '-->+' s2" := (exlab trans)^+ : lts_scope. 
-Notation "s1 '-->*' s2" := (exlab trans)^* : lts_scope.
+Prenex Implicits ltrans has_trans ftrans.
+
+Notation "s1 '--[' l ']-->' s2" := (ltrans l s1 s2) : lts_scope.
+Notation "s1 '-->' s2" := ((exlab ltrans) s1 s2) : lts_scope.
+Notation "s1 '-->?' s2" := ((exlab ltrans)^? s1 s2) : lts_scope.
+Notation "s1 '-->+' s2" := ((exlab ltrans)^+ s1 s2) : lts_scope. 
+Notation "s1 '-->*' s2" := ((exlab ltrans)^* s1 s2) : lts_scope.
+
+Section Theory.
+Context {L : Type} (S : ltsType L).
+Implicit Types (l : L) (s : S).
+
+Lemma ftrans_ltrans l s :
+  (s == ftrans l s) || (s --[l]--> ftrans l s).
+Proof. 
+  rewrite /ftrans; destruct idP; rewrite ?eq_refl //.
+  apply/orP; right; apply/xchooseP.
+Qed.
+
+Lemma ftrans_trans l s :
+  s -->? (ftrans l s).
+Proof. 
+  rewrite /= /dhrel_one. 
+  move: (ftrans_ltrans l s)=> /orP[].
+  - by move=> /eqP {1}->; left. 
+  by move=> ?; right; exists l. 
+Qed.
+
+Lemma has_ftrans l s : 
+  has_trans l s -> (s --[l]--> ftrans l s).
+Proof. rewrite /ftrans; destruct idP=> // _; apply/xchooseP. Qed. 
+
+End Theory.
 
 End LTS.
+
+
+Module Export dLTS.
+
+Module dLTS.
+Section ClassDef. 
+
+Record mixin_of (S0 : Type) (L : Type)
+                (sb : LTS.class_of S0 L)
+                (S := LTS.Pack sb) := Mixin {
+  _ : forall (l : L) (s1 s2 s3 : S), 
+        (s1 --[l]--> s2) -> (s1 --[l]--> s3) -> s2 = s3
+}.
+
+Set Primitive Projections.
+Record class_of (S : Type) (L : Type) := Class {
+  base  : LTS.class_of S L;
+  mixin : mixin_of base;
+}.
+Unset Primitive Projections.
+
+Local Coercion base : class_of >-> LTS.class_of.
+
+Structure type (L : Type) := Pack { sort; _ : class_of sort L }.
+
+Local Coercion sort : type >-> Sortclass.
+
+Variables (S : Type) (L : Type) (cT : type L).
+
+Definition class := let: Pack _ c as cT' := cT return class_of (sort cT') L in c.
+Definition clone c of phant_id class c := @Pack S c.
+
+Definition pack :=
+  fun bS b & phant_id (@LTS.class bS) b =>
+  fun m => Pack (@Class S L b m).
+
+Definition eqType := @Equality.Pack cT class.
+Definition choiceType := @Choice.Pack cT class.
+Definition countType := @Countable.Pack cT class.
+Definition ltsType := @LTS.Pack L cT class.
+
+End ClassDef.
+
+Module Export Exports.
+Coercion base : class_of >-> LTS.class_of.
+Coercion mixin : class_of >-> mixin_of.
+Coercion sort : type >-> Sortclass.
+Coercion eqType : type >-> Equality.type.
+Coercion choiceType : type >-> Choice.type.
+Coercion countType : type >-> Countable.type.
+Coercion ltsType : type >-> LTS.type.
+Canonical eqType.
+Canonical choiceType.
+Canonical countType.
+Canonical ltsType.
+End Exports.
+
+End dLTS.
+
+Export dLTS.Exports.
+
+Notation dltsType := dLTS.type.
+Notation dLTSType S L m := (@dLTS.pack S L _ _ id m).
+
+Section Theory.
+Context {L : Type} {S : dltsType L}.
+Implicit Types (l : L) (s : S).
+
+Lemma ltrans_det l s1 s2 s3 : 
+  (s1 --[l]--> s2) -> (s1 --[l]--> s3) -> s2 = s3.
+Proof. rewrite /ltrans; move: s1 s2 s3; case: S=> ? [? [H]]; exact/H. Qed.
+
+Lemma ltransE l s s' : 
+  (s --[l]--> s') = (has_trans l s) && (s' == ftrans l s).
+Proof. 
+  apply/idP/idP; last first.
+  - move=> /andP[] /[swap] /eqP {1}->; exact/has_ftrans.
+  move=> Htr; rewrite andb_idr=> [|?].
+  - by apply/has_transP; exists s'.
+  by apply/eqP/(ltrans_det Htr)/has_ftrans.
+Qed. 
+
+End Theory.
+
+End dLTS.
+
 
 (* Context {L : Type} {S : ltsType L}. *)
 (* Variable (l : L) (s1 s2 : S). *)
@@ -183,18 +347,21 @@ Canonical step_subType := Eval hnf in [subType for step_val].
 Definition step_of l s s' : (s --[l]--> s') -> step := 
   fun p => @Step (mk_step l s s') p.
 
-Definition adj : rel step := 
+Definition adj : rel stepTuple := 
   fun st st' => dst st == src st'. 
 
 End Def.
 
 Prenex Implicits lbl src dst is_step step_of adj.
 
-Section EQ. 
-Context {L : eqType} (S : ltsType L).
+Section Prod. 
+Context {L : Type} (S : ltsType L).
 
 Definition prod_of_step : stepTuple S -> L * S * S := 
   fun s => (lbl s, src s, dst s).
+
+Definition step_of_prod : L * S * S -> stepTuple S := 
+  fun '(lbl, src, dst) => mk_step lbl src dst.
 
 Lemma prod_of_step_inj : injective prod_of_step.
 Proof. 
@@ -202,17 +369,55 @@ Proof.
   by case x; case y=> /= ?????? -> -> ->. 
 Qed.
 
-Definition stepTuple_eqMixin := InjEqMixin prod_of_step_inj.
+Lemma prod_of_stepK : 
+  cancel prod_of_step step_of_prod.
+Proof. by case. Qed.
+
+End Prod.
+
+Section EQ.
+Context {L : eqType} (S : ltsType L).
+
+Definition stepTuple_eqMixin := InjEqMixin (@prod_of_step_inj L S).
 Canonical stepTuple_eqType := 
   Eval hnf in EqType (stepTuple S) stepTuple_eqMixin.
 
 Definition step_eqMixin := Eval hnf in [eqMixin of step S by <:].
 Canonical step_eqType := Eval hnf in EqType (step S) step_eqMixin.
 
-(* Variables (st1 st2 : step S). *)
-(* Check (st1 == st2). *)
-
 End EQ.
+
+Section Choice.
+Context {L : choiceType} (S : ltsType L).
+
+Definition stepTuple_choiceMixin := 
+  CanChoiceMixin (@prod_of_stepK L S).
+Canonical stepTuple_choiceType := 
+  Eval hnf in ChoiceType (stepTuple S) stepTuple_choiceMixin.
+
+Definition step_choiceMixin := 
+  Eval hnf in [choiceMixin of step S by <:].
+Canonical step_choiceType := 
+  Eval hnf in ChoiceType (step S) step_choiceMixin.
+
+End Choice.
+
+Section Countable.
+Context {L : countType} (S : ltsType L).
+
+Definition stepTuple_countMixin := 
+  CanCountMixin (@prod_of_stepK L S).
+Canonical stepTuple_countType := 
+  Eval hnf in CountType (stepTuple S) stepTuple_countMixin.
+
+Definition step_countMixin := 
+  Eval hnf in [countMixin of step S by <:].
+Canonical step_countType := 
+  Eval hnf in CountType (step S) step_countMixin.
+
+Canonical step_subCountType := [subCountType of (step S)].
+
+End Countable.
 
 Section Theory.
 Context {L : eqType} (S : ltsType L).
@@ -229,13 +434,13 @@ End Step.
 
 Module Export Trace. 
 
-Notation traceSeq S := (seq (step S)).
+Notation traceSeq S := (seq (stepTuple S)).
 
 Section Def. 
 Context {L : Type} (S : ltsType L).
 
 Definition is_trace : pred (traceSeq S) := 
-  fun ts => sorted adj ts.
+  fun ts => all is_step ts && sorted adj ts.
 
 Structure trace : Type := Trace { 
   trace_val :> traceSeq S; 
@@ -246,14 +451,22 @@ Canonical trace_subType := Eval hnf in [subType for trace_val].
 
 Implicit Types (ts : traceSeq S) (tr : trace).
 
-Definition labels : traceSeq S -> seq L := map (lbl : step S -> L). 
+Definition labels : traceSeq S -> seq L := map lbl. 
 
 Definition states : S -> traceSeq S -> seq S := 
   fun s ts => 
     match ts with 
     | [::]    => [:: s] 
-    | st :: _ => src st :: map (dst : step S -> S) ts
+    | st :: _ => src st :: map dst ts
     end. 
+
+Fixpoint trace_from (s : S) (ls : seq L) : traceSeq S :=
+  match ls with
+  | [::]    => [::]
+  | l :: ls => 
+    let s' := ftrans l s in
+    mk_step l s s' :: (trace_from s' ls) 
+  end.
 
 (* TODO: try `starts_with` and `ends_with` predicates instead? *)
 Definition fst_state : S -> traceSeq S -> S := 
@@ -289,51 +502,72 @@ Arguments adjoint : simpl never.
 Notation "[ 'trace' 'of' tr ]" := (mk_trace (fun trP => @Trace _ _ tr trP))
   (at level 0, format "[ 'trace'  'of'  tr ]") : form_scope.
 
+Notation "[ 'trace::' st ]" := [trace of [:: val st]]
+  (at level 0, format "[ 'trace::'  st ]") : form_scope.
+
 Notation "[ 'trace' ]" := [trace of [::]]
   (at level 0, format "[ 'trace' ]") : form_scope.
+
+Notation "[ 'trace?' 'of' ts ]" := [trace of insubd [trace] ts]
+  (at level 0, format "[ 'trace?'  'of'  ts ]") : form_scope.
+
+Notation "[ 'trace' 'from' s 'by' ls ]" := [trace? of trace_from s ls]
+  (at level 0, format "[ 'trace'  'from' s  'by' ls ]") : form_scope.
 
 Notation "tr1 '<+>' tr2" := [trace of adjoin tr1 tr2]
   (at level 51, left associativity) : lts_scope.
 
-Notation "st '<+' tr" := [trace of adjoin [:: st] tr]
+Notation "st '<+' tr" := [trace of adjoin [:: val st] tr]
   (at level 49, right associativity) : lts_scope.
 
-Notation "tr '+>' st" := [trace of adjoin tr [:: st]]
+Notation "tr '+>' st" := [trace of adjoin tr [:: val st]]
   (at level 48, left associativity) : lts_scope.
-
 
 Section Build.
 Context {L : Type} (S : ltsType L).
 Implicit Types (st : step S) (ts : traceSeq S) (tr : trace S).
 
-Lemma nil_traceP : is_trace ([::] : seq (step S)).
+Lemma nil_traceP : is_trace ([::] : traceSeq S).
 Proof. done. Qed.
 Canonical nil_trace := Trace nil_traceP.
 
-Lemma singl_traceP st : is_trace [:: st].
-Proof. done. Qed.
+Lemma singl_traceP st : is_trace [:: val st].
+Proof. apply/andP; split=> //=; rewrite andbT; exact/(valP st). Qed.
 Canonical singl_trace st := Trace (singl_traceP st).
+
+Lemma insub_traceP ts : is_trace (insubd [trace] ts).
+Proof. by rewrite val_insubd; case: ifP. Qed.
+Canonical insub_trace ts := Trace (insub_traceP ts).
+
+Lemma val_insub_trace ts : 
+  is_trace ts -> [trace? of ts] = ts :> traceSeq S.
+Proof. by rewrite /= val_insubd=> ->. Qed.
 
 Lemma adjoin_traceP tr1 tr2 : is_trace (adjoin tr1 tr2).
 Proof. 
   case: tr1=> [ts1]; case: tr2=> [ts2] /=.
   rewrite /adjoin /is_trace. 
   case: ifP=> [|?] //.
+  move=> Hadj /andP[Hs1 Ha1] /andP[Hs2 Ha2].
+  apply/andP; split.
+  - by rewrite all_cat; apply/andP. 
+  move: Hadj Hs1 Ha1 Hs2 Ha2.
   case: ts1=> [|st1 {}ts1] //=; rewrite cat_path.
-  case: ts2=> [|st2 {}ts2] //= ???; [exact/andP | exact/and3P].
+  case: ts2=> [|st2 {}ts2] //= ?????; [exact/andP | exact/and3P].
 Qed.
 Canonical adjoin_trace tr1 tr2 := Trace (adjoin_traceP tr1 tr2).
 
+(* TODO: rename to `val_adjoin` *)
 Lemma adjoin_val tr1 tr2 : 
   adjoint tr1 tr2 -> tr1 <+> tr2 = tr1 ++ tr2 :> traceSeq S.
 Proof. by rewrite /adjoin /=; case: ifP. Qed.
 
 Lemma adjoin_cons_val st tr : 
-  adjoint [:: st] tr -> st <+ tr = st :: tr :> traceSeq S.
+  adjoint [trace:: st] tr -> st <+ tr = val st :: tr :> traceSeq S.
 Proof. by rewrite /adjoin /=; case: ifP. Qed.
 
 Lemma adjoin_rcons_val st tr : 
-  adjoint tr [:: st] -> tr +> st = rcons tr st :> traceSeq S.
+  adjoint tr [trace:: st] -> tr +> st = rcons tr (val st) :> traceSeq S.
 Proof. by rewrite /adjoin -cats1 /=; case: ifP. Qed.
 
 End Build.
@@ -346,12 +580,36 @@ Canonical trace_eqType := Eval hnf in EqType (trace S) trace_eqMixin.
 
 End EQ.
 
-Section Theory. 
-Context {L : Type} (S : ltsType L).
-Implicit Types (st : step S) (ts : traceSeq S) (tr : trace S).
+Section Choice.
+Context {L : choiceType} (S : ltsType L).
+
+Definition trace_choiceMixin := 
+  Eval hnf in [choiceMixin of trace S by <:].
+Canonical trace_choiceType := 
+  Eval hnf in ChoiceType (trace S) trace_choiceMixin.
+
+End Choice.
+
+Section Countable.
+Context {L : countType} (S : ltsType L).
+
+Definition trace_countMixin := 
+  Eval hnf in [countMixin of trace S by <:].
+Canonical trace_countType := 
+  Eval hnf in CountType (trace S) trace_countMixin.
+
+End Countable.
+
+Section LTSTheory. 
+Context {L : Type} {S : ltsType L}.
+Implicit Types (l : L) (ls : seq L) (s : S).
+Implicit Types (st : stepTuple S) (ts : traceSeq S) (tr : trace S).
 
 Lemma trace_adj tr : sorted adj tr.
-Proof. by case: tr. Qed.
+Proof. by move: (valP tr)=> /andP[]. Qed.
+
+Lemma trace_steps tr : all is_step tr.
+Proof. by move: (valP tr)=> /andP[]. Qed.
 
 Lemma fst_state_src st ts : 
   fst_state (src st) ts = src (head st ts).
@@ -412,29 +670,29 @@ Lemma adjoint_lastE ts st :
 Proof. done. Qed.
 
 Lemma is_trace_cons st ts : 
-  is_trace (st :: ts) = [&& is_trace ts & adjoint [:: st] ts].
+  is_trace (st :: ts) = [&& is_step st, is_trace ts & adjoint [:: st] ts].
 Proof. 
   rewrite /is_trace /adjoint /=.
-  case: ts=> [|st' {}ts] //=.
-  by rewrite andbC; apply/andb_id2l=> _.
+  case: ts=> [|st' {}ts]; rewrite ?andbT //=.
+  by rewrite [adj st st' && _]andbC !andbA /adj.
 Qed.
 
 Lemma is_trace_rcons ts st : 
-  is_trace (rcons ts st) = [&& is_trace ts & adjoint ts [:: st]].
+  is_trace (rcons ts st) = [&& is_step st, is_trace ts & adjoint ts [:: st]].
 Proof.
-  rewrite /is_trace /adjoint. 
+  rewrite /is_trace /adjoint all_rcons. 
   case: (lastP ts)=> [|{}ts st'] //=.
-  - by rewrite eq_refl.
-  rewrite lst_state_rcons (sorted_rcons st). 
-  by rewrite /nilp /adj size_rcons last_rcons /=.
+  - by rewrite eq_refl andbT.
+  rewrite lst_state_rcons (sorted_rcons st).
+  by rewrite /nilp /adj size_rcons last_rcons !andbA /=. 
 Qed.
 
 Lemma size_labels ts : 
   size (labels ts) = size ts.
 Proof. by rewrite /labels size_map. Qed.
 
-Lemma labels_rcons s st : 
-  labels (rcons s st) = rcons (labels s) (lbl st).
+Lemma labels_rcons ts st : 
+  labels (rcons ts st) = rcons (labels ts) (lbl st).
 Proof. by rewrite /labels map_rcons. Qed.
 
 Lemma labels_cat ts1 ts2 : 
@@ -461,7 +719,68 @@ Lemma adjoins0 tr :
   tr <+> [trace] = tr.
 Proof. by apply/val_inj=> /=; rewrite adjoin_val ?adjoints0 ?cats0 //=. Qed.
 
-End Theory.
+Lemma trace_from_fst_state s ls : 
+  s = fst_state s (trace_from s ls).
+Proof. by case: ls. Qed.
+
+Lemma trace_from_labels s ls : 
+  labels (trace_from s ls) = ls.
+Proof. by move: s; elim ls=> [|?? IH] ? //=; rewrite IH. Qed.
+
+Lemma trace_from_lts_lang s ls : 
+  is_trace (trace_from s ls) -> lts_lang s ls.
+Proof. 
+  move=> Htr; rewrite /lts_lang.
+  exists (Trace Htr)=> /=.
+  - rewrite /trace_lang /=.
+    exact/eqP/trace_from_fst_state.
+  by rewrite trace_from_labels.  
+Qed.
+
+End LTSTheory.
+
+Section dLTSTheory. 
+Context {L : Type} {S : dltsType L}.
+Implicit Types (l : L) (ls : seq L) (s : S).
+Implicit Types (st : stepTuple S) (ts : traceSeq S) (tr : trace S).
+
+Lemma trace_from_is_trace s ls : 
+  lts_lang s ls -> is_trace (trace_from s ls).
+Proof. 
+  rewrite /lts_lang /trace_lang=> [[]].
+  case=> /= [] ts; move: s ls. 
+  elim: ts=> [|st {}ts] /=. 
+  - by move=> ???? ->.
+  move=> IH s ls Htr /eqP Hs -> //=.
+  move: Htr; rewrite !is_trace_cons. 
+  move=> /and3P[Hst Htr Hadj]. 
+  have ->: ftrans (lbl st) s = dst st.
+  - move: Hst; rewrite /is_step Hs ltransE. 
+    by move=> /andP[_] /eqP->.
+  apply/and3P; split.
+  - rewrite /is_step Hs=> /=; exact/Hst. 
+  - by apply/IH=> //; rewrite -adjoint_firstE.
+  rewrite adjoint_firstE=> //=.
+  exact/eqP/trace_from_fst_state.
+Qed.
+
+Lemma trace_from_trace_lang s ls : 
+  lts_lang s ls -> trace_lang s [trace from s by ls].
+Proof. 
+  move=> ?; rewrite /trace_lang /= val_insub_trace. 
+  - by apply/eqP/trace_from_fst_state.
+  exact/trace_from_is_trace.
+Qed.
+
+Lemma dlts_langP s ls : 
+  reflect (lts_lang s ls) (is_trace (trace_from s ls)).
+Proof. 
+  apply/(equivP idP); split. 
+  - exact/trace_from_lts_lang. 
+  exact/trace_from_is_trace.
+Qed.
+
+End dLTSTheory.
 
 End Trace.
 
@@ -539,20 +858,20 @@ Proof.
   - by move=> [tr' []] ???; exists tr'.
   move: Htr Hh; elim/last_ind: tr=> [|{}tr st IH] /=.
   - by exists [trace] => /=.
-  rewrite is_trace_rcons=> /andP[Htr Hj].
+  rewrite is_trace_rcons=> /and3P[Hst Htr Hj].
   rewrite fst_state_rcons -fst_state_src. 
   case: (nilp tr)/nilP=> [->|Hnil] /=. 
-  - move: (valP st); rewrite /is_step=> /[swap] <- => Hs. 
+  - move: Hst; rewrite /is_step=> /[swap] <- => Hs. 
     move: (sim_step HR Hs)=> [s' HR' Hs'].
     pose st' := step_of Hs'. 
-    by exists [trace of [:: st']]. 
+    by exists [trace:: st']. 
   rewrite (fst_stateNnil t) // => Ht.
   move: (IH Htr Ht); clear IH. 
   move=> [tr' []] /[swap].
   rewrite !labels_rcons.    
   move: Hj; rewrite adjoint_lastE=> /eqP. 
-  rewrite (lst_stateNnil t (src st))=> // ->. 
-  move: (valP st); rewrite /is_step=> Hs Hlbl HRl.
+  rewrite (lst_stateNnil t (src st))=> // ->.
+  move: Hst; rewrite /is_step=> Hs Hlbl HRl.
   move: (sim_step HRl Hs)=> [s'].
   move=> HR' Hs' /eqP Hfst.
   have: ~~ nilp tr'.
@@ -560,9 +879,9 @@ Proof.
     by move: Hnil=> /nilP.
   move=> /nilP Hnil'.
   pose st' := step_of Hs'.
-  exists (tr' +> st')=> /=.
+  exists (tr' +> st'). 
   rewrite !adjoin_rcons_val; last first; [|split].
-  - by rewrite /adjoint step_of_val (lst_stateNnil s) /=. 
+  - by rewrite /adjoint /= (lst_stateNnil s) /=.  
   - by rewrite !lst_state_rcons /=.
   - by rewrite labels_rcons Hlbl.
   rewrite fst_state_rcons Hfst -fst_state_src. 
